proof/theories/Extract.v
@@ -34,4 +34,5 @@ Separate Extraction
   eval_ruleset
   run_ruleset
   set_env
-  seq_eval.
+  seq_eval
+  env_with_sets.
